Lp2lc/Active/Util.lean
@@ -58,8 +58,6 @@ def isSemiDecidable : (self : Outcome T) → Prop
 
 end Outcome
 
-def ByteCode := String
-
 universe u v
 
 -- 1. Implicitly lift a type to a higher universe using ULift
