Tests/DOT/Sanity.lean
@@ -13,85 +13,86 @@ namespace Tests.DOT.Sanity
 open Lp2lc.Active.DOT
 open Lp2lc.Active.Util
 
-private def emptyBody {I : Type} : ObjectBody I :=
+private def emptyBody {I : Type} {ByteCode : Type} : ObjectBody I ByteCode :=
   { lookup := fun _ => none }
 
-private def singletonBody {I : Type} (name : Name) (entry : MemberImpl I) :
-    ObjectBody I :=
+private def singletonBody {I : Type} {ByteCode : Type} (name : Name) (entry : MemberImpl I ByteCode) :
+    ObjectBody I ByteCode :=
   { lookup := fun key => if key = name then some entry else none }
 
-private def namedTermImpl {I : Type} (name : Name) (body : Trm I) (annotation : Typ I) :
-    MemberImpl I :=
+private def namedTermImpl {I : Type} {ByteCode : Type} (name : Name)
+    (body : Trm I ByteCode) (annotation : Typ I ByteCode) :
+    MemberImpl I ByteCode :=
   .term (some name) body annotation
 
-private def implicitSubtypeEntry {I : Type} (tUnder tOver : Typ I) :
-    MemberDeclaration I :=
+private def implicitSubtypeEntry {I : Type} {ByteCode : Type} (tUnder tOver : Typ I ByteCode) :
+    MemberDeclaration I ByteCode :=
   .term none true (.evidence (.subtypeEv tUnder tOver))
 
-private def selfMemberTyp {I : Type} (this : I) (name : Name) : Typ I :=
+private def selfMemberTyp {I : Type} {ByteCode : Type} (this : I) (name : Name) : Typ I ByteCode :=
   .depSelectTyp (.var this .top) name
 
 namespace Trm
 
-def false : TrmClosed :=
+def false : TrmClosed String :=
   .val (.primitive "false")
 
-def true : TrmClosed :=
+def true : TrmClosed String :=
   .val (.primitive "true")
 
-def identityFn : TrmClosed :=
+def identityFn : TrmClosed String :=
   .val
     (.depFn (fun x => .var x .primitive))
 
-def identityFnOnFalse : TrmClosed :=
+def identityFnOnFalse : TrmClosed String :=
   .depApply identityFn false
 
-def get1st : TrmClosed :=
+def get1st : TrmClosed String :=
   .val
     (.depFn (fun x =>
       .val
         (.depFn (fun _y => .var x .primitive))))
 
-def get2nd : TrmClosed :=
+def get2nd : TrmClosed String :=
   .val
     (.depFn (fun _x =>
       .val
         (.depFn (fun y => .var y .primitive))))
 
-def get1stOnTuple : TrmClosed :=
+def get1stOnTuple : TrmClosed String :=
   .depApply
     (.depApply get1st false)
     true
 
-def get2ndOnTuple : TrmClosed :=
+def get2ndOnTuple : TrmClosed String :=
   .depApply
     (.depApply get2nd false)
     true
 
-def apply1stOn2ndFn : TrmClosed :=
+def apply1stOn2ndFn : TrmClosed String :=
   .val (.depFn (fun f =>
     .val (.depFn (fun x =>
       .depApply
         (.var f (.depFn .primitive (fun _ => .primitive)))
         (.var x .primitive)))))
 
-def apply1stOn2ndFnOnTuple : TrmClosed :=
+def apply1stOn2ndFnOnTuple : TrmClosed String :=
   .depApply
     (.depApply apply1stOn2ndFn identityFn)
     false
 
-def structural1Trm : TrmClosed :=
+def structural1Trm : TrmClosed String :=
   .val
     (.object (fun _this =>
       singletonBody "a"
         (namedTermImpl "a" (.val (.primitive "false")) .primitive)))
 
-def structural1Typ : TrmClosed :=
+def structural1Typ : TrmClosed String :=
   .val
     (.object (fun _this =>
       singletonBody "A" (.typeAlias "A")))
 
-def structural1Bounded : TrmClosed :=
+def structural1Bounded : TrmClosed String :=
   .val
     (.object (fun _this =>
       emptyBody))
@@ -100,54 +101,54 @@ end Trm
 
 namespace Typ
 
-def false : TypClosed :=
+def false : TypClosed String :=
   .primitive
 
-def true : TypClosed :=
+def true : TypClosed String :=
   .primitive
 
-def identityFn : TypClosed :=
+def identityFn : TypClosed String :=
   .depFn .primitive (fun _x => .primitive)
 
-def identityFnOnFalse : TypClosed :=
+def identityFnOnFalse : TypClosed String :=
   .primitive
 
-def get1st : TypClosed :=
+def get1st : TypClosed String :=
   .depFn .primitive (fun _x =>
     .depFn .primitive (fun _y => .primitive))
 
-def get2nd : TypClosed :=
+def get2nd : TypClosed String :=
   .depFn .primitive (fun _x =>
     .depFn .primitive (fun _y => .primitive))
 
-def get1stOnTuple : TypClosed :=
+def get1stOnTuple : TypClosed String :=
   .primitive
 
-def get2ndOnTuple : TypClosed :=
+def get2ndOnTuple : TypClosed String :=
   .primitive
 
-def apply1stOn2ndFn : TypClosed :=
+def apply1stOn2ndFn : TypClosed String :=
   .depFn
     (.depFn .primitive (fun _x => .primitive))
     (fun _f =>
       .depFn .primitive (fun _x => .primitive))
 
-def apply1stOn2ndFnOnTuple : TypClosed :=
+def apply1stOn2ndFnOnTuple : TypClosed String :=
   .primitive
 
-def structural1Trm : TypClosed :=
+def structural1Trm : TypClosed String :=
   .selfBinder (fun _this =>
     .oneMember (.term (some "a") Bool.false .primitive))
 
-def structural1Typ : TypClosed :=
+def structural1Typ : TypClosed String :=
   .selfBinder (fun _this =>
     .oneMember (.typeAlias "A"))
 
-def emptyTrait : TypClosed :=
+def emptyTrait : TypClosed String :=
   .selfBinder (fun _this =>
     .oneMember (.typeAlias "class_EmptyTrait"))
 
-def structural1Bounded : TypClosed :=
+def structural1Bounded : TypClosed String :=
   .selfBinder (fun this =>
     .and
       (.oneMember (.typeAlias "A"))
@@ -159,7 +160,7 @@ def structural1Bounded : TypClosed :=
             (selfMemberTyp this "A")
             emptyTrait))))
 
-def subTrait : TypClosed :=
+def subTrait : TypClosed String :=
   .selfBinder (fun this =>
     .and
       (.oneMember (.typeAlias "class_EmptyTrait"))
